nonlinear: prove universal atn analytic regularity

candle/cv_compute_analytic_expr_calculus.ml
@@ -33,7 +33,10 @@ let candle_analytic_valid_dim_def = define
      candle_analytic_valid_dim n a) /\
   (candle_analytic_valid_dim n
       (Candle_analytic_sqrt lp ln ld up un ud a) <=>
-     candle_analytic_valid_dim n a)`;;
+     candle_analytic_valid_dim n a) /\
+  (candle_analytic_valid_dim n (Candle_analytic_atn a) <=>
+     candle_analytic_valid_dim n a) /\
+  (candle_analytic_valid_dim n Candle_analytic_pi_half <=> T)`;;
 
 let candle_analytic_regular_at_def = define
  `(candle_analytic_regular_at env (Candle_analytic_poly p) <=> T) /\
@@ -51,7 +54,10 @@ let candle_analytic_regular_at_def = define
   (candle_analytic_regular_at env
       (Candle_analytic_sqrt lp ln ld up un ud a) <=>
      candle_analytic_regular_at env a /\
-     &0 < candle_analytic_value env a)`;;
+     &0 < candle_analytic_value env a) /\
+  (candle_analytic_regular_at env (Candle_analytic_atn a) <=>
+     candle_analytic_regular_at env a) /\
+  (candle_analytic_regular_at env Candle_analytic_pi_half <=> T)`;;
 
 let candle_analytic_denote_dim_def = new_definition
  `candle_analytic_denote_dim e (z:real^N) =
@@ -111,6 +117,19 @@ let candle_analytic_denote_dim_sqrt = prove
      (candle_analytic_denote_dim
        (Candle_analytic_sqrt lp ln ld up un ud a) : real^N->real) =
      (\z. sqrt (candle_analytic_denote_dim a z))`,
+  REWRITE_TAC[FUN_EQ_THM; candle_analytic_denote_dim_def;
+              candle_analytic_value_def]);;
+
+let candle_analytic_denote_dim_atn = prove
+ (`!a. (candle_analytic_denote_dim (Candle_analytic_atn a) :
+         real^N->real) =
+       (\z. atn (candle_analytic_denote_dim a z))`,
+  REWRITE_TAC[FUN_EQ_THM; candle_analytic_denote_dim_def;
+              candle_analytic_value_def]);;
+
+let candle_analytic_denote_dim_pi_half = prove
+ (`(candle_analytic_denote_dim Candle_analytic_pi_half : real^N->real) =
+   (\z. pi / &2)`,
   REWRITE_TAC[FUN_EQ_THM; candle_analytic_denote_dim_def;
               candle_analytic_value_def]);;
 
@@ -306,6 +325,33 @@ let candle_analytic_denote_dim_diff2c = prove
                  `(candle_analytic_denote_dim a):real^N->real`]
                 diff2c_sqrt_compose)
               regular)
-            source)))]);;
+            source)));
+    X_GEN_TAC `a:candle_analytic_expr` THEN DISCH_THEN
+      (LABEL_TAC "ih") THEN X_GEN_TAC `z:real^N` THEN
+    REWRITE_TAC[candle_analytic_valid_dim_def;
+                candle_analytic_regular_at_def] THEN STRIP_TAC THEN
+    REWRITE_TAC[candle_analytic_denote_dim_atn] THEN
+    USE_THEN "ih" (fun ih ->
+      let source =
+        MATCH_MP (SPEC `z:real^N` ih)
+          (CONJ
+            (ASSUME `candle_analytic_valid_dim (dimindex (:N)) a`)
+            (ASSUME
+              `candle_analytic_regular_at
+                (list_of_seq (\k. (z:real^N)$(k + 1))
+                  (dimindex (:N))) a`)) in
+      ACCEPT_TAC
+        (REWRITE_RULE[o_DEF]
+          (MATCH_MP
+            (SPECL
+              [`z:real^N`;
+               `(candle_analytic_denote_dim a):real^N->real`]
+              diff2c_atn_compose)
+            source)));
+    X_GEN_TAC `z:real^N` THEN
+    REWRITE_TAC[candle_analytic_valid_dim_def;
+                candle_analytic_regular_at_def;
+                candle_analytic_denote_dim_pi_half] THEN
+    MATCH_ACCEPT_TAC diff2c_const]);;
 
 end;;
